<?xml version="1.0" encoding="UTF-8"?>
<!--
	======================================================================
	Created:     23.11.2008
	Version:     $Id: ProfileServiceTermination.owl,v 1.1 2011/01/24 06:37:55 nick Exp $

   (c) 2009 Thorsten Möller - University of Basel Switzerland

   The MIT License
   Permission is hereby granted, free of charge, to any person obtaining a copy
   of this software and associated documentation files (the "Software"), to
   deal in the Software without restriction, including without limitation the
   rights to use, copy, modify, merge, publish, distribute, sublicense, and/or
   sell copies of the Software, and to permit persons to whom the Software is
   furnished to do so, subject to the following conditions:

   The above copyright notice and this permission notice shall be included in
   all copies or substantial portions of the Software.

   THE SOFTWARE IS PROVIDED "AS IS", WITHOUT WARRANTY OF ANY KIND, EXPRESS OR
   IMPLIED, INCLUDING BUT NOT LIMITED TO THE WARRANTIES OF MERCHANTABILITY,
   FITNESS FOR A PARTICULAR PURPOSE AND NONINFRINGEMENT. IN NO EVENT SHALL THE
   AUTHORS OR COPYRIGHT HOLDERS BE LIABLE FOR ANY CLAIM, DAMAGES OR OTHER
   LIABILITY, WHETHER IN AN ACTION OF CONTRACT, TORT OR OTHERWISE, ARISING
   FROM, OUT OF OR IN CONNECTION WITH THE SOFTWARE OR THE USE OR OTHER DEALINGS
   IN THE SOFTWARE.

	======================================================================
-->
<!DOCTYPE uridef[
  <!ENTITY rdf "http://www.w3.org/1999/02/22-rdf-syntax-ns">
  <!ENTITY rdfs "http://www.w3.org/2000/01/rdf-schema">
  <!ENTITY owl "http://www.w3.org/2002/07/owl">
  <!ENTITY xsd "http://www.w3.org/2001/XMLSchema">
  <!ENTITY dc  "http://purl.org/dc/elements/1.1/">
  <!ENTITY shadow-rdf "http://www.daml.org/services/owl-s/1.2/generic/ObjectList.owl">
  <!ENTITY profile "http://www.daml.org/services/owl-s/1.2/Profile.owl">
  <!ENTITY service-param "http://www.daml.org/services/owl-s/1.2/ServiceParameter.owl">
  <!ENTITY THIS "http://on.cs.unibas.ch/owl-s/1.2/ProfileServiceTermination.owl">
]>

<rdf:RDF
  xmlns:rdf=	  "&rdf;#"
  xmlns:shadow-rdf= "&shadow-rdf;#"
  xmlns:rdfs=	  "&rdfs;#"
  xmlns:owl =    "&owl;#"
  xmlns:profile= "&profile;#"
  xmlns:service-param= "&service-param;#"
  xmlns:dc=      "&dc;#"
  xmlns=	        "&THIS;#"
  xml:base=      "&THIS;">

<owl:Ontology rdf:about="">
	<rdfs:comment xml:lang="en">
		Extension to the OWL-S profile ontology that can be used to express
		termination properties about a service. This is achieved by extending
		the service Profile concept. Services annotated by such information
		enable transactional processes that offer rollback respectively
		compensation means.

		TODO: add link to corresponding publication.
	</rdfs:comment>
	<owl:versionInfo>$Id: ProfileServiceTermination.owl,v 1.1 2011/01/24 06:37:55 nick Exp $</owl:versionInfo>
	<dc:creator>Thorsten Möller</dc:creator>
	<dc:date>2009-06-20</dc:date>
	<dc:rights>
		Copyright 2009 Thorsten Möller - University of Basel Switzerland
	</dc:rights>
	<owl:imports rdf:resource="&profile;" />
	<owl:imports rdf:resource="&service-param;" />
</owl:Ontology>


<!--######################################################
    Compensation related properties and concepts
    ######################################################-->

<owl:ObjectProperty rdf:ID="compensator">
	<rdfs:comment xml:lang="en">
		Used to model if and by whom some service can be compensated, that is,
		whether another service exists that either semantically undoes the
		effects created by the subject service, or by any other kind of
		compensation operation. The latter would not necessarily have to undo
		the effects but may create new effects that are defined to represent a
		compensation. In other words, compensation subsumes rollback (i.e. the
		inverse operation).
	</rdfs:comment>
	<rdfs:subPropertyOf rdf:resource="&service-param;#serviceParameter" />
	<rdfs:range rdf:resource="#CompensationServiceParameter" />
</owl:ObjectProperty>

<owl:Class rdf:ID="CompensationServiceParameter">
	<rdfs:comment xml:lang="en">
		Specialized service parameter used to specify the compensation profile(s)
		of some profile.

		Since profiles always correspond to some service one can also say that this
		parameter relates some service to its compensation service(s).
	</rdfs:comment>
	<rdfs:subClassOf rdf:resource="&service-param;#ServiceParameter" />
	<rdfs:subClassOf>
		<owl:Restriction>
			<rdfs:comment xml:lang="en">
				Limit range of sParameter to compensator service Profiles.
			</rdfs:comment>
			<owl:onProperty rdf:resource="&service-param;#sParameter" />
			<owl:allValuesFrom rdf:resource="#Compensator" />
		</owl:Restriction>
	</rdfs:subClassOf>
</owl:Class>

<owl:Class rdf:ID="Compensatable">
	<rdfs:comment xml:lang="en">
		A service profile for which at least one compensation service does exist.
	</rdfs:comment>
	<rdfs:subClassOf rdf:resource="&profile;#Profile" />
	<rdfs:subClassOf>
		<owl:Restriction>
			<rdfs:comment xml:lang="en">
				Make compensator property mandatory, i.e., one or more.
			</rdfs:comment>
			<owl:onProperty rdf:resource="#compensator" />
			<owl:minCardinality rdf:datatype="&xsd;#nonNegativeInteger">1</owl:minCardinality>
		</owl:Restriction>
	</rdfs:subClassOf>
</owl:Class>

<owl:Class rdf:ID="Pivot">
	<rdfs:comment xml:lang="en">
		A service profile for which a compensation service does not exist.
	</rdfs:comment>
	<rdfs:subClassOf rdf:resource="&profile;#Profile" />
	<owl:complementOf rdf:resource="#Compensatable" />
	<owl:equivalentClass>
		<owl:Restriction>
			<rdfs:comment xml:lang="en">
				Pivot services are characterized by the fact that they can not be
				compensated, which is the case if no compensator exists. Note that
				when reasoning using the OWA it can actually never be inferred if
				something is pivot based on this restriction. This is only possible
				using CWA.
			</rdfs:comment>
			<owl:onProperty rdf:resource="#compensator" />
			<owl:cardinality rdf:datatype="&xsd;#nonNegativeInteger">0</owl:cardinality>
		</owl:Restriction>
	</owl:equivalentClass>
</owl:Class>


<!--######################################################
    Retriability related properties and concepts
    ######################################################-->

<owl:ObjectProperty rdf:ID="retriable">
	<rdfs:comment xml:lang="en">
		Used to model that some service is guaranteed to successfully terminate
		after a finite number of invocations, that is, its failure probability
		equals zero. For instance, services that realize some idempotent
		operation are intrinsically retriable.
	</rdfs:comment>
	<rdfs:subPropertyOf rdf:resource="&service-param;#serviceParameter" />
	<rdfs:range rdf:resource="#RetriabilityServiceParameter" />
</owl:ObjectProperty>

<owl:Class rdf:ID="RetriabilityServiceParameter">
	<rdfs:comment xml:lang="en">
		Specialized service parameter used to specify if some service may be
		re-invoked in case its termination failed.

		Since services always specify to at least one profile it is o.k. to speak
		about the service here even though this class is used with the service
		Profile.
	</rdfs:comment>
	<rdfs:subClassOf rdf:resource="&service-param;#ServiceParameter" />
	<rdfs:subClassOf>
		<owl:Restriction>
			<rdfs:comment xml:lang="en">
				Limit range of sParameter to service booleans.
			</rdfs:comment>
			<owl:onProperty rdf:resource="&service-param;#sParameter" />
			<owl:allValuesFrom rdf:resource="#Boolean" />
		</owl:Restriction>
	</rdfs:subClassOf>
</owl:Class>

<owl:Class rdf:ID="Retriable">
	<rdfs:comment xml:lang="en">
		A service profile which can be re-invoked in case of unsuccessful
		termination.
	</rdfs:comment>
	<rdfs:subClassOf rdf:resource="&profile;#Profile" />
	<owl:equivalentClass>
		<owl:Restriction>
			<rdfs:comment xml:lang="en">
				Everything that has the property #retriable set to #True is retriable.
			</rdfs:comment>
			<owl:onProperty rdf:resource="#retriable" />
			<owl:hasValue rdf:resource="#True" />
		</owl:Restriction>
	</owl:equivalentClass>
</owl:Class>

<owl:Class rdf:ID="NonRetriable">
	<rdfs:comment xml:lang="en">
		A service profile which can not be re-invoked in case of unsuccessful
		termination.
	</rdfs:comment>
	<rdfs:subClassOf rdf:resource="&profile;#Profile" />
	<owl:complementOf rdf:resource="#Retriable" />
	<owl:equivalentClass>
		<owl:Restriction>
			<rdfs:comment xml:lang="en">
				Everything that has the property #retriable set to #False is non retriable.
			</rdfs:comment>
			<owl:onProperty rdf:resource="#retriable" />
			<owl:hasValue rdf:resource="#False" />
		</owl:Restriction>
	</owl:equivalentClass>
</owl:Class>


<!--######################################################
    Derived class Compensator
    ######################################################-->

<owl:Class rdf:ID="Compensator">
	<rdfs:comment xml:lang="en">
		A service profile which represents the compensation operation for some
		service.
	</rdfs:comment>
	<owl:intersectionOf rdf:parseType="Collection">
		<owl:Class rdf:about="#Retriable" />
		<owl:Class rdf:about="#Pivot" />
	</owl:intersectionOf>
</owl:Class>

<!--<profile:Profile rdf:ID="TestCompensatable">-->
<!--	<compensator>-->
<!--		<CompensationServiceParameter>-->
<!--			<service-param:sParameter rdf:resource="#TestCompensator" />-->
<!--		</CompensationServiceParameter>-->
<!--	</compensator>-->
<!--	<retriable>-->
<!--		<RetriabilityServiceParameter>-->
<!--			<service-param:sParameter rdf:resource="#True" />-->
<!--		</RetriabilityServiceParameter>-->
<!--	</retriable>-->
<!--</profile:Profile>-->
<!---->
<!--<Compensator rdf:ID="TestCompensator" />-->
<!---->
<!--<Pivot rdf:ID="Test1" />-->
<!--<Pivot rdf:ID="Test" />-->
<!--<Retriable rdf:about="#Test" />-->


<!--######################################################
    Helper classes and individuals
    ######################################################-->

<owl:Class rdf:ID="Boolean">
	<rdfs:comment xml:lang="en">
		We need this class because the "serviceParameter" property is an object
		property, hence, its sub property "retriable" also needs to refer to
		individuals and not data values.

		REFACTOR: If there is a well established public ontology that specifies the
		same concept we may either remove it here, or (which seems to be the more
		elegant way) add additional axioms that express that the concepts are
		equivalent. In the same way it might be possible then to specify that the
		the two individuals True and False are the same as individuals declared
		in the external ontology.
	</rdfs:comment>
	<owl:oneOf rdf:parseType="Collection">
		<Boolean rdf:about="#True" />
		<Boolean rdf:about="#False" />
	</owl:oneOf>
</owl:Class>

<owl:AllDifferent>
	<owl:distinctMembers rdf:parseType="Collection">
		<Boolean rdf:about="#True" />
		<Boolean rdf:about="#False" />
	</owl:distinctMembers>
</owl:AllDifferent>

</rdf:RDF>


