<?xml version='1.0' encoding="UTF-8"?>
<!DOCTYPE uridef [
	<!ENTITY rdf 		"http://www.w3.org/1999/02/22-rdf-syntax-ns">
	<!ENTITY rdfs 		"http://www.w3.org/2000/01/rdf-schema">
	<!ENTITY owl 		"http://www.w3.org/2002/07/owl">
	<!ENTITY xsd 		"http://www.w3.org/2001/XMLSchema">
	<!ENTITY service 	"http://www.daml.org/services/owl-s/1.1/Service.owl">
	<!ENTITY profile 	"http://www.daml.org/services/owl-s/1.1/Profile.owl">
	<!ENTITY process 	"http://www.daml.org/services/owl-s/1.1/Process.owl">
	<!ENTITY grounding 	"http://www.daml.org/services/owl-s/1.1/Grounding.owl">
]>

<rdf:RDF
  xmlns:rdf = "&rdf;#" 
  xmlns:rdfs = "&rdfs;#" 
  xmlns:owl = "&owl;#" 
  xmlns:xsd = "&xsd;#" 
  xmlns:service = "&service;#" 
  xmlns:profile = "&profile;#" 
  xmlns:process = "&process;#" 
  xmlns:grounding ="&grounding;#" 
  xml:base=		"http://www.ifi.unizh.ch/ddis/ont/owl-s/MoreGroundings.owl" > 
<owl:Ontology rdf:about="">
	<rdfs:comment>
		Upper-Level Ontology for extended groundings for the OWL-S 1.1 service markup language.
	</rdfs:comment>
	<owl:versionInfo>$Id: MoreGroundings.owl,v 1.1 2011/01/24 06:37:51 nick Exp $</owl:versionInfo> 	
	
	<owl:imports rdf:resource="&process;"/>
	<owl:imports rdf:resource="&service;"/>
	<owl:imports rdf:resource="&grounding;"/>
</owl:Ontology>
		
<!-- ****************************************************************************** -->
							<!--  JavaGrounding  -->
<!-- ****************************************************************************** -->
<owl:Class rdf:ID="JavaGrounding">
	<rdfs:comment>A JavaGrounding is a collection of JavaAtomicProcessGrounding instances</rdfs:comment>
	<rdfs:subClassOf rdf:resource="&service;#ServiceGrounding"/>		
</owl:Class>
  
<owl:ObjectProperty rdf:ID="hasAtomicProcessGrounding"> 
	<rdfs:comment>Expands domain and range of grounding#hasJavaAtomicProcessGrounding</rdfs:comment>  
	<rdfs:domain rdf:resource="#JavaGrounding"/>
	<rdfs:range rdf:resource="#JavaAtomicProcessGrounding"/>
</owl:ObjectProperty>

<!-- JavaAtomicProcessGrounding -->
<owl:Class rdf:ID="JavaAtomicProcessGrounding">
	<rdfs:comment>This class binds an OWL-S Process to a single, specific Java method</rdfs:comment>	
	<rdfs:subClassOf>
		<owl:Restriction>
			<owl:onProperty rdf:resource="#javaClass"/>
			<owl:minCardinality rdf:datatype="&xsd;#nonNegativeInteger">1</owl:minCardinality>  
		</owl:Restriction>
	</rdfs:subClassOf>	
	<rdfs:subClassOf>
		<owl:Restriction>
			<owl:onProperty rdf:resource="#javaMethod"/>
			<owl:minCardinality rdf:datatype="&xsd;#nonNegativeInteger">1</owl:minCardinality>  
		</owl:Restriction>
	</rdfs:subClassOf>	
</owl:Class>	
  
<owl:ObjectProperty rdf:ID="owlsProcess">
	<rdfs:comment>The atomic process to which this grounding applies.</rdfs:comment>
	<rdfs:domain rdf:resource="#JavaAtomicProcessGrounding"/>
	<rdfs:range rdf:resource="&process;#AtomicProcess"/>
</owl:ObjectProperty>
<owl:FunctionalProperty rdf:about="#owlsProcess"/>
  
<owl:DatatypeProperty rdf:ID="javaClass">
	<rdfs:comment>Fully qualified class-name, in which method is located</rdfs:comment>
	<rdfs:domain rdf:resource="#JavaAtomicProcessGrounding"/>
	<rdfs:range rdf:resource="&xsd;#string"/>
</owl:DatatypeProperty>
	
<owl:DatatypeProperty rdf:ID="javaMethod">
	<rdfs:comment>name of method to invoke</rdfs:comment>
	<rdfs:domain rdf:resource="#JavaAtomicProcessGrounding"/>
	<rdfs:range rdf:resource="&xsd;#string"/>
</owl:DatatypeProperty>
	
<owl:ObjectProperty rdf:ID="javaOutput">
	<rdfs:comment>reference to JavaType, which will be used as output variable</rdfs:comment>
	<rdfs:domain rdf:resource="#JavaAtomicProcessGrounding"/>
	<rdfs:range rdf:resource="#JavaVariable"/>
</owl:ObjectProperty>

<owl:ObjectProperty rdf:ID="hasJavaParameter">
	<rdfs:domain rdf:resource="#JavaAtomicProcessGrounding"/>
	<rdfs:range rdf:resource="#JavaParameter"/>
</owl:ObjectProperty>  

<owl:Class rdf:ID="JavaVariable">
  	<rdfs:comment>This represents the mapping from a OWLS-Parameter to a Java type</rdfs:comment>
  	<rdfs:subClassOf>
    	<owl:Restriction>
        	<owl:onProperty rdf:resource="#javaType"/>
        	<owl:cardinality rdf:datatype="&xsd;#nonNegativeInteger">1</owl:cardinality>  
      </owl:Restriction>
    </rdfs:subClassOf>	
    <rdfs:subClassOf>
    	<owl:Restriction>
    		<owl:onProperty rdf:resource="#owlsParameter"/>
			<owl:cardinality rdf:datatype="&xsd;#nonNegativeInteger">1</owl:cardinality>  
		</owl:Restriction>
	</rdfs:subClassOf>	
</owl:Class>
	    
<owl:DatatypeProperty rdf:ID="javaType">
  	<rdfs:comment>The corresponding Java type for the OWL-S Parameter</rdfs:comment>
	<rdfs:domain rdf:resource="#JavaVariable"/>
	<rdfs:range rdf:resource="&xsd;#string"/>
</owl:DatatypeProperty>
	
<owl:ObjectProperty rdf:ID="owlsParameter">
	<rdfs:comment>Adds #JavaVariable to the domain of #owlsParameter</rdfs:comment>
	<rdfs:domain rdf:resource="#JavaVariable"/>
	<rdfs:range rdf:resource="&process;#Parameter"/>
</owl:ObjectProperty>

<owl:DatatypeProperty rdf:ID="transformatorClass">
	<rdfs:comment>Links to the class that transforms java objects from/to OWL individuals</rdfs:comment>
	<rdfs:domain rdf:resource="#JavaVariable"/>
	<rdfs:range rdf:resource="&xsd;#string"/>
</owl:DatatypeProperty>
	
<owl:Class rdf:ID="JavaParameter">
	<rdfs:comment>This defines the mapping from a OWLS-Parameter to a JavaParameter</rdfs:comment>			  
	<rdfs:subClassOf rdf:resource="#JavaVariable"/>
	<rdfs:subClassOf>
    	<owl:Restriction>
			<owl:onProperty rdf:resource="#paramIndex"/>
			<owl:cardinality rdf:datatype="&xsd;#nonNegativeInteger">1</owl:cardinality>  
		</owl:Restriction>
	</rdfs:subClassOf>		    
</owl:Class>
 	
<owl:DatatypeProperty rdf:ID="paramIndex">
	<rdfs:comment>Index in parameter list of Java method signature</rdfs:comment>
	<rdfs:domain rdf:resource="#JavaParameter"/>
	<rdfs:range rdf:resource="&xsd;#nonNegativeInteger"/>
</owl:DatatypeProperty>

</rdf:RDF>